\xiaosi


\begin{equation}
     \sum_{i=\left\lceil\frac{m}{2}\right\rceil}^{m}\left(\begin{array}{c}
     m \\
     i
     \end{array}\right) p^{i}(1-p)^{m-i}=\sum_{i=0}^{\left\lfloor\frac{m}{2}\right\rfloor}\left(\begin{array}{c}
     m \\
     i
     \end{array}\right)(1-p)^{i} p^{m-i}
\end{equation}


\begin{equation}
    \begin{aligned}
        \operatorname{Pr}\left\{o_{k}^{*} \!\succeq \!r\! \succeq \!o_{c k}^{*} \mid x, m\right\}\!=\!1 & \!-\!\sum_{i=\left\lceil\frac{m}{2}\right\rceil}^{m}\!\left(\!\begin{array}{c}
        m \\
        i
        \end{array}\right) p^{i}(1\!-\!p)^{m\!-\!i} \\
        & \!-\!\sum_{i=\left\lceil\frac{m+1}{2}\right\rceil}^{m}\!\left(\!\begin{array}{c}
        m \\
        i
        \end{array}\right) q^{m\!-\!i}(1\!-\!q)^{i}
    \end{aligned}
\end{equation}